Make induction rules for new iterate_norms.

Isabelle/Grammar_defs.thy
@@ -104,6 +104,10 @@ definition itno_invariant_sd_in where
   "itno_invariant_sd_in norms rules n t vs \<equiv>
      t_rules_have_norm norms rules \<and> (n, t, vs) = min_norm_of_t_rules norms rules"
 
+definition itno2_invariant_sd_in where
+  "itno2_invariant_sd_in norms rules norm \<equiv>
+     t_rules_have_norm norms rules \<and> norm = min_norm_of_t_rules norms rules"
+
 definition gram_normed_fun :: "('t :: linorder, 'v :: linorder) grammar \<Rightarrow> bool" where
   "gram_normed_fun gr \<equiv> snd (iterate_norms gr) = []"
 
